feat(data/list/sort): implement merge sort and prove correctness

data/list/sort.lean
@@ -3,9 +3,37 @@ Copyright (c) 2016 Jeremy Avigad. All rights reserved.
 Released under Apache 2.0 license as described in the file LICENSE.
 Author: Jeremy Avigad
 
-Sorting for lists.
+Insertion sort and merge sort.
 -/
 import .perm
+
+-- TODO(Jeremy): move this
+
+namespace nat
+
+theorem add_pos_left {m : ℕ} (h : m > 0) (n : ℕ) : m + n > 0 :=
+calc
+  m + n > 0 + n : nat.add_lt_add_right h n
+    ... = n     : nat.zero_add n
+    ... ≥ 0     : zero_le n
+
+theorem add_pos_right (m : ℕ) {n : ℕ} (h : n > 0) : m + n > 0 :=
+begin rw add_comm, exact add_pos_left h m end
+
+theorem add_pos_iff_pos_or_pos (m n : ℕ) : m + n > 0 ↔ m > 0 ∨ n > 0 :=
+iff.intro
+  begin
+    intro h,
+    cases m with m,
+    {rw nat.zero_add at h, exact or.inr h},
+    exact or.inl (succ_pos _)
+  end
+  begin
+    intro h, cases h with mpos npos,
+    { apply add_pos_left mpos },
+    apply add_pos_right _ npos
+  end
+end nat
 
 namespace list
 
@@ -41,8 +69,7 @@ end sorted
 
 section sort
 universe variable uu
-parameters {α : Type uu} [decidable_eq α]
-parameters (r : α → α → Prop) [decidable_rel r]
+parameters {α : Type uu} (r : α → α → Prop) [decidable_rel r]
 local infix `≼` : 50 := r
 
 /- insertion sort -/
@@ -53,39 +80,38 @@ def ordered_insert (a : α) : list α → list α
 | []       := [a]
 | (b :: l) := if a ≼ b then a :: (b :: l) else b :: ordered_insert l
 
+attribute [simp] ordered_insert.equations.eqn_1 ordered_insert.equations.eqn_2
+
 def insertion_sort : list α → list α
 | []       := []
 | (b :: l) := ordered_insert b (insertion_sort l)
 
-end insertion_sort
+attribute [simp] insertion_sort.equations.eqn_1 insertion_sort.equations.eqn_2
 
 section correctness
+parameter [deceqα : decidable_eq α]
+include deceqα
 open perm
 
--- TODO(Jeremy): I tried to add [decidable_eq α] here, but Lean complained
--- that _inst_1 was already declared
+-- TODO(Jeremy): anonymous type class parameters don't work well
+-- TODO(Jeremy): in all the proofs below, simp [if_pos h] doesn't work
 
 theorem count_ordered_insert_eq (b a : α) : ∀ l, count b (ordered_insert a l) = count b (a :: l)
-| []       := by simp [ordered_insert.equations.eqn_1]
-| (c :: l) := decidable.by_cases
-                (suppose a ≼ c,
-                  by rw [ordered_insert.equations.eqn_2, if_pos this])
-                (suppose ¬ a ≼ c,
-                  begin
-                    rw [ordered_insert.equations.eqn_2, if_neg this],
-                    simp [count_cons', count_ordered_insert_eq]
-                  end)
+| []       := by simp
+| (c :: l) := if h : a ≼ c then
+                begin simp, rw [if_pos h] end
+              else
+                begin
+                  simp, rw [if_neg h], simp [count_cons', count_ordered_insert_eq]
+                end
 
-theorem mem_ordered_insert (b a : α) (l : list α) : b ∈ ordered_insert a l ↔ b ∈ a :: l :=
+theorem mem_ordered_insert_iff (b a : α) (l : list α) : b ∈ ordered_insert a l ↔ b ∈ a :: l :=
 by simp [mem_iff_count_pos, count_ordered_insert_eq]
 
 theorem perm_insertion_sort : ∀ l, insertion_sort l ~ l
 | []       := take a, rfl
 | (b :: l) := take a,
-              begin
-                rw [insertion_sort.equations.eqn_2, count_ordered_insert_eq],
-                simp [count_cons', perm_insertion_sort l a]
-              end
+              by simp [count_ordered_insert_eq, count_cons', perm_insertion_sort l a]
 
 section total_and_transitive
 variables (totr : total r) (transr : transitive r)
@@ -97,31 +123,30 @@ theorem sorted_ordered_insert (a : α) : ∀ l, sorted r l → sorted r (ordered
   assume h,
   have sorted r l, from sorted_of_sorted_cons r h,
   have h₀ : ∀ c ∈ l, b ≼ c, from forall_mem_rel_of_sorted_cons r h,
-  decidable.by_cases
-   (suppose a ≼ b,
-     begin
-       rw [ordered_insert.equations.eqn_2, if_pos this],
-       have ∀ c ∈ b :: l, a ≼ c, from
-         take c, suppose c ∈ b :: l,
-         or.elim (eq_or_mem_of_mem_cons this)
-           (suppose c = b, this^.symm ▸ ‹a ≼ b›)
-           (suppose c ∈ l, transr ‹a ≼ b› (h₀ _ this)),
-       sorted_cons r h this
-     end)
-   (suppose ¬ a ≼ b,
-     have b ≼ a, from or.resolve_left (totr a b) this,
-     begin
-       rw [ordered_insert.equations.eqn_2, if_neg ‹¬ a ≼ b›],
-       have h₁ : sorted r (ordered_insert r a l), from sorted_ordered_insert l ‹sorted r l›,
-       have h₂ : ∀ c ∈ ordered_insert r a l, b ≼ c, from
-         take c,
-         suppose c ∈ ordered_insert r a l,
-         have c ∈ a  :: l, from (mem_ordered_insert r c a l)^.mp this,
-         or.elim (eq_or_mem_of_mem_cons this)
-           (suppose c = a, begin rw this, exact ‹b ≼ a› end)
-           (suppose c ∈ l, h₀ c this),
-       show sorted r (b :: ordered_insert r a l), from sorted_cons r h₁ h₂
-     end)
+  if h' : a ≼ b then
+    begin
+      simp, rw [if_pos h'],
+      have ∀ c ∈ b :: l, a ≼ c, from
+        take c, suppose c ∈ b :: l,
+        or.elim (eq_or_mem_of_mem_cons this)
+          (suppose c = b, this^.symm ▸ ‹a ≼ b›)
+          (suppose c ∈ l, transr ‹a ≼ b› (h₀ _ this)),
+      show sorted r (a :: b :: l), from sorted_cons r h this
+   end
+  else
+    have b ≼ a, from or.resolve_left (totr a b) h',
+    begin
+      simp, rw [if_neg ‹¬ a ≼ b›],
+      have h₁ : sorted r (ordered_insert r a l), from sorted_ordered_insert l ‹sorted r l›,
+      have h₂ : ∀ c ∈ ordered_insert r a l, b ≼ c, from
+        take c,
+        suppose c ∈ ordered_insert r a l,
+        have c ∈ a  :: l, from (mem_ordered_insert_iff r c a l)^.mp this,
+        or.elim (eq_or_mem_of_mem_cons this)
+          (suppose c = a, begin rw this, exact ‹b ≼ a› end)
+          (suppose c ∈ l, h₀ c this),
+      show sorted r (b :: ordered_insert r a l), from sorted_cons r h₁ h₂
+    end
 
 theorem sorted_insert_sort : ∀ l, sorted r (insertion_sort l)
 | []       := sorted_nil r
@@ -129,10 +154,261 @@ theorem sorted_insert_sort : ∀ l, sorted r (insertion_sort l)
 
 end total_and_transitive
 end correctness
+end insertion_sort
+
+/- merge sort -/
+
+section merge_sort
+
+-- TODO(Jeremy): observation: if instead we write (a :: (split l).1, b :: (split l).2), the
+-- equation compiler can't prove the third equation
+
+def split : list α → list α × list α
+| []            := ([], [])
+| [a]           := ([a], [])
+| (a :: b :: l) := match split l with
+                   | (l₁, l₂) := (a :: l₁, b :: l₂)
+                   end
+
+-- TODO(Jeremy): the cases is needed because the internal split_match gets a pair
+
+theorem split_cons_cons (a b : α) (l : list α) :
+  split (a :: b :: l) = (a :: (split l).1, b :: (split l).2) :=
+begin rw [split.equations.eqn_3], cases split l, reflexivity end
+
+attribute [simp] split.equations.eqn_1 split.equations.eqn_2 split_cons_cons
+
+theorem length_split_fst_le : ∀ l : list α, length ((split l).1) ≤ length l
+| [] := nat.le_refl 0
+| [a] := nat.le_refl 1
+| (a :: b :: l) := begin
+                     simp, rw [add_comm],
+                     transitivity,
+                     apply add_le_add_right (length_split_fst_le l),
+                     apply nat.le_succ
+                   end
+
+theorem length_split_snd_le : ∀ l : list α, length ((split l).2) ≤ length l
+| [] := nat.le_refl 0
+| [a] := nat.zero_le 1
+| (a :: b :: l) := begin
+                     simp, rw [add_comm],
+                     transitivity,
+                     apply add_le_add_right (length_split_snd_le l),
+                     apply nat.le_succ
+                   end
+
+theorem length_split_cons_cons_fst_lt (a b : α) (l : list α) :
+  length (split (a :: b :: l)).1 < length (a :: b :: l) :=
+begin
+  simp, rw [add_comm],
+  exact add_lt_add_of_le_of_lt (length_split_fst_le l) (nat.le_refl _)
+end
+
+theorem length_split_cons_cons_snd_lt (a b : α) (l : list α) :
+  length (split (a :: b :: l)).2 < length (a :: b :: l) :=
+begin
+  simp, rw [add_comm],
+  exact add_lt_add_of_le_of_lt (length_split_snd_le l) (nat.le_refl _)
+end
+
+-- Do the well-founded recursion by hand, until the function definition system supports it.
+
+private def merge.F :
+  Π p : list α × list α,
+      (Π p₁ : list α × list α, length p₁.1 + length p₁.2 < length p.1 + length p.2 → list α) →
+    list α
+| ([], l)           f := l
+| (a :: l, [])      f := a :: l
+| (a :: l, b :: l') f := if a ≼ b then
+                            a :: f (l, b :: l') begin simp, apply nat.le_refl end
+                          else
+                            b :: f (a :: l, l') begin simp, apply nat.le_refl end
+
+def merge := well_founded.fix (inv_image.wf _ nat.lt_wf) merge.F
+
+theorem merge.def (p : list α × list α) : merge p = merge.F p (λ p h, merge p) :=
+well_founded.fix_eq (inv_image.wf _ nat.lt_wf) merge.F p
+
+@[simp]
+theorem merge.equations.eq_1 (l : list α) : merge ([], l) = l :=
+begin rw merge.def, reflexivity end
+
+@[simp]
+theorem merge.equations.eq_2 (a : α) (l : list α) : merge (a :: l, []) = a :: l :=
+begin rw merge.def, reflexivity end
+
+@[simp]
+theorem merge.equations.eq_3 (a b : α) (l l' : list α) :
+  merge (a :: l, b :: l') = if a ≼ b then
+                             a :: merge (l, b :: l')
+                           else
+                             b :: merge (a :: l, l') :=
+begin rw merge.def, reflexivity end
+
+private def merge_sort.F :
+  Π l : list α, (Π l₁ : list α, length l₁ < length l → list α) → list α
+| []            f := []
+| [a]           f := [a]
+| (a :: b :: l) f := let p  := split (a :: b :: l),
+                         l₁ := f p.1 (length_split_cons_cons_fst_lt a b l),
+                         l₂ := f p.2 (length_split_cons_cons_snd_lt a b l) in
+                     merge (l₁, l₂)
+
+def merge_sort := well_founded.fix (inv_image.wf _ nat.lt_wf) merge_sort.F
+
+theorem merge_sort.def (l : list α) : merge_sort l = merge_sort.F l (λ l h, merge_sort l) :=
+well_founded.fix_eq (inv_image.wf _ nat.lt_wf) merge_sort.F l
+
+@[simp]
+theorem merge_sort.equations.eq_1 : merge_sort [] = [] :=
+begin rw merge_sort.def, reflexivity end
+
+@[simp]
+theorem merge_sort.equations.eq_2 (a : α) : merge_sort [a] = [a] :=
+begin rw merge_sort.def, reflexivity end
+
+@[simp]
+theorem merge_sort.equations.eq_3 (a b : α) (l : list α) :
+  merge_sort (a :: b :: l) = let p := split (a :: b :: l) in
+                             merge (merge_sort p.1, merge_sort p.2) :=
+begin rw merge_sort.def, reflexivity end
+
+section correctness
+parameter [deceqα : decidable_eq α]
+include deceqα
+
+-- TODO(Jeremy): note that simp has to be called twice in the beginning, to reduce projections
+theorem count_split (a : α) : ∀ l : list α, count a (split l).1 + count a (split l).2 = count a l
+| []            := rfl
+| [a]           := rfl
+| (a :: b :: l) := begin simp, simp, simp [count_cons'], rw [-count_split l], simp end
+
+private def count_merge.F (c : α) :
+  Π p : list α × list α,
+      (Π p₁ : list α × list α, length p₁.1 + length p₁.2 < length p.1 + length p.2 →
+        count c (merge p₁) = count c p₁.1 + count c p₁.2) →
+    count c (merge p) = count c p.1 + count c p.2
+| ([], l)            f := by simp
+| (a :: l, [])       f := by simp
+| (a :: l, b :: l')  f := if h : a ≼ b then
+                            begin
+                              note hrec := f (l, b :: l') begin simp, apply nat.le_refl end,
+                              simp, rw [if_pos h], simp [count_cons', hrec]
+                            end
+                          else
+                            begin
+                              note hrec := f (a :: l, l') begin simp, apply nat.le_refl end,
+                              simp, rw [if_neg h], simp [count_cons', hrec]
+                            end
+
+theorem count_merge (c : α) :
+  ∀ p : list α × list α, count c (merge p) = count c p.1 + count c p.2 :=
+well_founded.fix (inv_image.wf _ nat.lt_wf) (count_merge.F c)
+
+theorem mem_merge_iff (a : α) (p : list α × list α) : a ∈ merge p ↔ a ∈ p.1 ∨ a ∈ p.2 :=
+by simp [mem_iff_count_pos, count_merge, nat.add_pos_iff_pos_or_pos]
+
+private def perm_merge_sort.F :
+  Π l : list α, (Π l₁ : list α, length l₁ < length l → merge_sort l₁ ~ l₁) →
+    merge_sort l ~ l
+| []  f           := take c, rfl
+| [a] f           := take c, rfl
+| (a :: b :: l) f :=
+  begin
+    intro c,
+    pose hrec₁ := f _ (length_split_cons_cons_fst_lt a b l) c,
+    pose hrec₂ := f _ (length_split_cons_cons_snd_lt a b l) c,
+    simp at hrec₁, simp at hrec₁, simp at hrec₂, simp at hrec₂,
+    simp [hrec₁, hrec₂, count_merge, count_split, count_cons']
+  end
+
+theorem perm_merge_sort : ∀ l : list α, merge_sort l ~ l :=
+well_founded.fix (inv_image.wf _ nat.lt_wf) perm_merge_sort.F
+
+section total_and_transitive
+variables (totr : total r) (transr : transitive r)
+include totr transr
+
+private def sorted_merge.F :
+  Π p : list α × list α,
+      (Π p₁ : list α × list α, length p₁.1 + length p₁.2 < length p.1 + length p.2 →
+        (sorted r p₁.1 → sorted r p₁.2 → sorted r (merge p₁))) →
+    sorted r p.1 → sorted r p.2 → sorted r (merge p)
+| ([], l)           f h₁ h₂ := begin simp, exact h₂ end
+| (a :: l, [])      f h₁ h₂ := begin simp, exact h₁ end
+| (a :: l, b :: l') f h₁ h₂ :=
+  have sorted r l, from sorted_of_sorted_cons r h₁,
+  have sorted r l', from sorted_of_sorted_cons r h₂,
+  have h₁₀ : ∀ c ∈ l, a ≼ c, from forall_mem_rel_of_sorted_cons r h₁,
+  have h₂₀ : ∀ c ∈ l', b ≼ c, from forall_mem_rel_of_sorted_cons r h₂,
+  if h : a ≼ b then
+    begin
+      note hrec := f (l, b :: l') begin simp, apply nat.le_refl end,
+      simp, rw [if_pos h],
+      have h₃ : sorted r (merge r (l, b :: l')), from hrec ‹sorted r l› h₂,
+      have h₄ : ∀ c ∈ merge r (l, b :: l'), a ≼ c,
+      begin
+        intros c hc,
+        rw mem_merge_iff at hc,
+        exact or.elim hc
+          (suppose c ∈ l, show a ≼ c, from h₁₀ c this)
+          (suppose c ∈ b :: l',
+            or.elim (eq_or_mem_of_mem_cons this)
+              (suppose c = b, show a ≼ c, from this^.symm ▸ ‹a ≼ b›)
+              (suppose c ∈ l', show a ≼ c, from transr ‹a ≼ b› (h₂₀ c this)))
+      end,
+      show sorted r (a :: merge r (l, b :: l')), from sorted_cons r h₃ h₄
+    end
+  else
+    have h' : b ≼ a, from or.resolve_left (totr a b) h,
+    begin
+      note hrec := f (a :: l, l') begin simp, apply nat.le_refl end,
+      simp, rw [if_neg h],
+      have h₃ : sorted r (merge r (a :: l, l')), from hrec h₁ ‹sorted r l'›,
+      have h₄ : ∀ c ∈ merge r (a :: l, l'), b ≼ c,
+      begin
+        intros c hc,
+        rw mem_merge_iff at hc,
+        exact or.elim hc
+          (suppose c ∈ a :: l,
+            or.elim (eq_or_mem_of_mem_cons this)
+              (suppose c = a, show b ≼ c, from this^.symm ▸ ‹b ≼ a›)
+              (suppose c ∈ l, show b ≼ c, from transr ‹b ≼ a› (h₁₀ c this)))
+          (suppose c ∈ l', show b ≼ c, from h₂₀ c this)
+      end,
+      show sorted r (b :: merge r (a :: l, l')), from sorted_cons r h₃ h₄
+    end
+
+theorem sorted_merge : Π {p : list α × list α},
+  sorted r p.1 → sorted r p.2 → sorted r (merge p) :=
+well_founded.fix (inv_image.wf _ nat.lt_wf) (sorted_merge.F totr transr)
+
+private def sorted_merge_sort.F :
+  Π l : list α, (Π l₁ : list α, length l₁ < length l → sorted r (merge_sort l₁)) →
+    sorted r (merge_sort l)
+| []            f := sorted_nil r
+| [a]           f := sorted_singleton r a
+| (a :: b :: l) f :=
+  begin
+    simp,
+    apply sorted_merge r totr transr,
+    { apply f, exact length_split_cons_cons_fst_lt a b l },
+    apply f, exact length_split_cons_cons_snd_lt a b l
+  end
+
+theorem sorted_merge_sort : ∀ l : list α, sorted r (merge_sort l) :=
+well_founded.fix (inv_image.wf _ nat.lt_wf) (sorted_merge_sort.F totr transr)
+
+end total_and_transitive
+end correctness
+end merge_sort
 end sort
 
-/- try it out! -/
+/- try them out! -/
 
 vm_eval insertion_sort (λ m n : ℕ, m ≤ n) [5, 27, 221, 95, 17, 43, 7, 2, 98, 567, 23, 12]
+
+vm_eval merge_sort     (λ m n : ℕ, m ≤ n) [5, 27, 221, 95, 17, 43, 7, 2, 98, 567, 23, 12]
 
 end list
